wip

code/bignum/Hacl.Bignum.GenericField.fst
@@ -25,27 +25,27 @@ friend Hacl.Spec.Bignum.GenericField
 
 #set-options "--z3rlimit 50 --fuel 1 --ifuel 0"
 
-let bn_field_get_len k _ =
+let bn_field_get_len #t k _ =
   k.len
 
 
-let bn_field_init km r nBits n =
+let bn_field_init #t km r nBits n =
   [@inline_let]
   let len = km.BM.bn.BN.len in
   let h0 = ST.get () in
-  let r2 : buffer (limb U64) = LowStar.Monotonic.Buffer.mmalloc r (uint #U64 #SEC 0) len in
-  let n1 : buffer (limb U64) = LowStar.Monotonic.Buffer.mmalloc r (uint #U64 #SEC 0) len in
+  let r2 : buffer (limb t) = LowStar.Monotonic.Buffer.mmalloc r (uint #t #SEC 0) len in
+  let n1 : buffer (limb t) = LowStar.Monotonic.Buffer.mmalloc r (uint #t #SEC 0) len in
   let h1 = ST.get () in
   B.(modifies_only_not_unused_in loc_none h0 h1);
   assert (B.length r2 == FStar.UInt32.v len);
   assert (B.length n1 == FStar.UInt32.v len);
-  let r2 : lbignum U64 len = r2 in
-  let n1 : lbignum U64 len = n1 in
+  let r2 : lbignum t len = r2 in
+  let n1 : lbignum t len = n1 in
   copy n1 n;
 
   km.BM.precomp (nBits -! 1ul) n r2;
   let mu = BM.mod_inv_limb n.(0ul) in
-  let res : bn_mont_ctx = { nBits = nBits; len = len; n = n1; mu = mu; r2 = r2 } in
+  let res : bn_mont_ctx t = { nBits = nBits; len = len; n = n1; mu = mu; r2 = r2 } in
   let h2 = ST.get () in
   assert (as_ctx h2 res == S.bn_field_init (v nBits) (as_seq h0 n));
   assert (S.bn_mont_ctx_inv (as_ctx h2 res));
@@ -53,83 +53,75 @@ let bn_field_init km r nBits n =
   res
 
 
-let bn_to_field km k a aM =
+let bn_to_field #t km k a aM =
   let h0 = ST.get () in
   km.BM.to k.n k.mu k.r2 a aM;
   let h1 = ST.get () in
-  assert (as_seq h1 aM == S.bn_to_field (as_ctx h0 k) (as_seq h0 a));
-  assert (bn_v h1 aM < bn_v h0 k.n)
+  assert (as_seq h1 aM == S.bn_to_field (as_ctx h0 k) (as_seq h0 a))
 
 
-let bn_from_field km k aM a =
+let bn_from_field #t km k aM a =
   let h0 = ST.get () in
   km.BM.from k.n k.mu aM a;
   let h1 = ST.get () in
-  assert (as_seq h1 a == S.bn_from_field (as_ctx h0 k) (as_seq h0 aM));
-  assert (bn_v h1 a < bn_v h0 k.n)
+  assert (as_seq h1 a == S.bn_from_field (as_ctx h0 k) (as_seq h0 aM))
 
 
-let bn_field_add km k aM bM cM =
+let bn_field_add #t km k aM bM cM =
   let h0 = ST.get () in
   km.BM.bn.BN.add_mod_n k.n aM bM cM;
   let h1 = ST.get () in
-  assert (as_seq h1 cM == S.bn_field_add (as_ctx h0 k) (as_seq h0 aM) (as_seq h0 bM));
-  assert (bn_v h1 cM < bn_v h0 k.n)
+  assert (as_seq h1 cM == S.bn_field_add (as_ctx h0 k) (as_seq h0 aM) (as_seq h0 bM))
 
 
-let bn_field_sub km k aM bM cM =
+let bn_field_sub #t km k aM bM cM =
   let h0 = ST.get () in
   BN.bn_sub_mod_n k.len k.n aM bM cM;
   let h1 = ST.get () in
-  assert (as_seq h1 cM == S.bn_field_sub (as_ctx h0 k) (as_seq h0 aM) (as_seq h0 bM));
-  assert (bn_v h1 cM < bn_v h0 k.n)
+  assert (as_seq h1 cM == S.bn_field_sub (as_ctx h0 k) (as_seq h0 aM) (as_seq h0 bM))
 
 
-let bn_field_mul km k aM bM cM =
+let bn_field_mul #t km k aM bM cM =
   let h0 = ST.get () in
   km.BM.mul k.n k.mu aM bM cM;
   let h1 = ST.get () in
-  assert (as_seq h1 cM == S.bn_field_mul (as_ctx h0 k) (as_seq h0 aM) (as_seq h0 bM));
-  assert (bn_v h1 cM < bn_v h0 k.n)
+  assert (as_seq h1 cM == S.bn_field_mul (as_ctx h0 k) (as_seq h0 aM) (as_seq h0 bM))
 
 
-let bn_field_sqr km k aM cM =
+let bn_field_sqr #t km k aM cM =
   let h0 = ST.get () in
   km.BM.sqr k.n k.mu aM cM;
   let h1 = ST.get () in
-  assert (as_seq h1 cM == S.bn_field_sqr (as_ctx h0 k) (as_seq h0 aM));
-  assert (bn_v h1 cM < bn_v h0 k.n)
+  assert (as_seq h1 cM == S.bn_field_sqr (as_ctx h0 k) (as_seq h0 aM))
 
 
-let bn_field_one km k oneM =
+let bn_field_one #t km k oneM =
   let h0 = ST.get () in
   BM.bn_mont_one km k.n k.mu k.r2 oneM;
   let h1 = ST.get () in
-  assert (as_seq h1 oneM == S.bn_field_one (as_ctx h0 k));
-  assert (bn_v h1 oneM < bn_v h0 k.n)
+  assert (as_seq h1 oneM == S.bn_field_one (as_ctx h0 k))
 
 
-let bn_field_inv km k aM aInvM =
+let bn_field_inv #t km k aM aInvM =
   [@inline_let]
   let len = k.len in
   push_frame ();
-  let n2 = create len (uint #U64 #SEC 0) in
-  let c = BN.bn_sub1 len k.n (uint #U64 #SEC 2) n2 in
+  let n2 = create len (uint #t #SEC 0) in
+  let c = BN.bn_sub1 len k.n (uint #t #SEC 2) n2 in
   let h0 = ST.get () in
   S.bn_field_inv_lemma (as_ctx h0 k) (as_seq h0 aM);
-  Hacl.Spec.Bignum.bn_sub1_lemma (as_seq h0 k.n) (uint #U64 #SEC 2);
+  Hacl.Spec.Bignum.bn_sub1_lemma (as_seq h0 (k.n <: lbignum t len)) (uint #t #SEC 2);
   Hacl.Spec.Bignum.Definitions.bn_eval_bound (as_seq h0 n2) (v len);
-  Hacl.Spec.Bignum.Definitions.bn_eval_bound (as_seq h0 k.n) (v len);
+  Hacl.Spec.Bignum.Definitions.bn_eval_bound (as_seq h0 (k.n <: lbignum t len)) (v len);
   BE.bn_mont_one km k.n k.mu k.r2 aInvM;
-  IE.lexp_fw_vartime len len (BE.mk_lexp U64 km ((as_ctx h0 k).S.n) k.mu) k.n aM len k.nBits n2 aInvM 4ul;
+  IE.lexp_fw_vartime len len (BE.mk_lexp t km ((as_ctx h0 k).S.n) k.mu) k.n aM len k.nBits n2 aInvM 4ul;
   let h1 = ST.get () in
-  assert (bn_v h0 n2 == bn_v h0 k.n - 2);
+  assert (bn_v h0 n2 == bn_v #t #k.len h0 k.n - 2);
   assert (as_seq h1 aInvM ==
     Lib.Exponentiation.exp_fw
     (Hacl.Spec.Bignum.Exponentiation.mk_bn_mont_comm_monoid ((as_ctx h0 k).S.n) k.mu)
-    (as_seq h0 aM) (v k.nBits) (bn_v h0 k.n - 2) 4);
+    (as_seq h0 aM) (v k.nBits) (bn_v #t #k.len h0 k.n - 2) 4);
 
   norm_spec [delta_only [`%S.bn_field_inv]] (S.bn_field_inv (as_ctx h0 k) (as_seq h0 aM));
   assert (as_seq h1 aInvM == S.bn_field_inv (as_ctx h0 k) (as_seq h0 aM));
-  assert (bn_v h1 aInvM < bn_v h0 k.n);
   pop_frame ()
