code/bignum/Hacl.Bignum.GenericField.fsti
@@ -21,210 +21,245 @@ module BM = Hacl.Bignum.Montgomery
 
 #set-options "--z3rlimit 50 --fuel 0 --ifuel 0"
 
+// from Jonathan:
+// type limb_t = U32 | U64
+// let f (x: t) = match x with | U32 -> lbuffer UInt32.t | U64 -> lbuffer UInt64.t
+// type ctx' (x: t) (a: Type0 { a == f x }) = {
+//   r2: a;
+// }
+// let ctx (x: t) = ctx' x (f x)
+
+inline_for_extraction noextract
+let lb (t:limb_t) =
+  match t with
+  | U32 -> buffer uint32
+  | U64 -> buffer uint64
+
+inline_for_extraction noextract
+let ll (t:limb_t) =
+  match t with
+  | U32 -> uint32
+  | U64 -> uint64
+
 //inline_for_extraction noextract
-class bn_mont_ctx = {
+noeq
+type bn_mont_ctx' (t:limb_t) (a:Type0{a == lb t}) (b:Type0{b == ll t}) = {
   nBits: size_t;
-  len: BN.meta_len U64;
-  n: lbignum U64 len;
-  mu: limb U64;
-  r2: lbignum U64 len;
+  len: BN.meta_len t;
+  n: x:a{length #MUT #(limb t) x == v len};
+  mu: b;
+  r2: x:a{length #MUT #(limb t) x == v len};
   }
 
 
+let bn_mont_ctx (t:limb_t) = bn_mont_ctx' t (lb t) (ll t)
+
+
 inline_for_extraction noextract
-let as_ctx (h:mem) (k:bn_mont_ctx) : GTot (S.bn_mont_ctx U64) = {
+let as_ctx (#t:limb_t) (h:mem) (k:bn_mont_ctx t) : GTot (S.bn_mont_ctx t) = {
   S.nBits = v k.nBits;
   S.len = v k.len;
-  S.n = as_seq h k.n;
+  S.n = as_seq h (k.n <: lbignum t k.len);
   S.mu = k.mu;
-  S.r2 = as_seq h k.r2;
+  S.r2 = as_seq h (k.r2 <: lbignum t k.len);
   }
 
 
 inline_for_extraction noextract
-let bn_mont_ctx_inv (h:mem) (k:bn_mont_ctx) =
-  live h k.n /\ live h k.r2 /\ disjoint k.n k.r2 /\
+let bn_mont_ctx_inv (#t:limb_t) (h:mem) (k:bn_mont_ctx t) =
+  live h (k.n <: lbignum t k.len) /\ live h (k.r2 <: lbignum t k.len) /\
+  disjoint (k.n <: lbignum t k.len) (k.r2 <: lbignum t k.len) /\
   S.bn_mont_ctx_inv (as_ctx h k)
 
 
 inline_for_extraction noextract
-let bn_field_get_len_st (k:bn_mont_ctx) = unit ->
-  Stack (BN.meta_len U64)
+let bn_field_get_len_st (#t:limb_t) (k:bn_mont_ctx t) = unit ->
+  Stack (BN.meta_len t)
   (requires fun h -> bn_mont_ctx_inv h k)
   (ensures  fun h0 r h1 -> h0 == h1 /\
     v r == S.bn_field_get_len (as_ctx h0 k))
 
 
 inline_for_extraction noextract
-val bn_field_get_len: k:bn_mont_ctx -> bn_field_get_len_st k
+val bn_field_get_len: #t:limb_t -> k:bn_mont_ctx t -> bn_field_get_len_st k
 
 
 inline_for_extraction noextract
-let bn_field_init_st (len:BN.meta_len U64) =
+let bn_field_init_st (t:limb_t) (len:BN.meta_len t) =
     r:HS.rid
   -> nBits:size_t
-  -> n:lbignum U64 len ->
-  ST (bn_mont_ctx)
+  -> n:lbignum t len ->
+  ST (bn_mont_ctx t)
   (requires fun h ->
     live h n /\ S.bn_mont_ctx_pre (v nBits) (v len) (as_seq h n) /\
     ST.is_eternal_region r)
   (ensures  fun h0 res h1 ->
     B.(modifies loc_none h0 h1) /\
     S.bn_mont_ctx_inv (as_ctx h1 res) /\
-    B.(fresh_loc (loc_union (loc_buffer (res.n <: buffer (limb U64))) (loc_buffer (res.r2 <: buffer (limb U64)))) h0 h1) /\
-    B.(loc_includes (loc_region_only false r) (loc_union (loc_buffer (res.n <: buffer (limb U64))) (loc_buffer (res.r2 <: buffer (limb U64))))) /\
+    B.(fresh_loc (loc_union (loc_buffer (res.n <: buffer (limb t))) (loc_buffer (res.r2 <: buffer (limb t)))) h0 h1) /\
+    B.(loc_includes (loc_region_only false r) (loc_union (loc_buffer (res.n <: buffer (limb t))) (loc_buffer (res.r2 <: buffer (limb t))))) /\
     as_ctx h1 res == S.bn_field_init (v nBits) (as_seq h0 n))
 
 
 inline_for_extraction noextract
-val bn_field_init: km:BM.mont U64 -> bn_field_init_st km.BM.bn.BN.len
+val bn_field_init: #t:limb_t -> km:BM.mont t -> bn_field_init_st t km.BM.bn.BN.len
 
 
 inline_for_extraction noextract
-let bn_to_field_st (k:bn_mont_ctx) =
-    a:lbignum U64 k.len
-  -> aM:lbignum U64 k.len ->
+let bn_to_field_st (#t:limb_t) (k:bn_mont_ctx t) =
+    a:lbignum t k.len
+  -> aM:lbignum t k.len ->
   Stack unit
   (requires fun h ->
     bn_mont_ctx_inv h k /\ live h a /\ live h aM /\ disjoint a aM /\
-    disjoint a k.r2 /\ disjoint a k.n /\
-    disjoint aM k.r2 /\ disjoint aM k.n /\
-    bn_v h a < bn_v h k.n)
+    disjoint a (k.r2 <: lbignum t k.len) /\ disjoint a (k.n <: lbignum t k.len) /\
+    disjoint aM (k.r2 <: lbignum t k.len) /\ disjoint aM (k.n <: lbignum t k.len) /\
+    bn_v h a < bn_v #t #k.len h k.n)
   (ensures  fun h0 _ h1 -> modifies (loc aM) h0 h1 /\
-    bn_v h1 aM < bn_v h0 k.n /\
+    bn_v h1 aM < bn_v #t #k.len h0 k.n /\
     as_seq h1 aM == S.bn_to_field (as_ctx h0 k) (as_seq h0 a))
 
 
 inline_for_extraction noextract
-val bn_to_field: km:BM.mont U64 -> k:bn_mont_ctx{k.len == km.BM.bn.BN.len} -> bn_to_field_st k
+val bn_to_field: #t:limb_t -> km:BM.mont t -> k:bn_mont_ctx t{k.len == km.BM.bn.BN.len} -> bn_to_field_st k
 
 
 inline_for_extraction noextract
-let bn_from_field_st (k:bn_mont_ctx) =
-    aM:lbignum U64 k.len
-  -> a:lbignum U64 k.len ->
+let bn_from_field_st (#t:limb_t) (k:bn_mont_ctx t) =
+    aM:lbignum t k.len
+  -> a:lbignum t k.len ->
   Stack unit
   (requires fun h ->
     bn_mont_ctx_inv h k /\ live h a /\ live h aM /\ disjoint a aM /\
-    disjoint a k.r2 /\ disjoint a k.n /\
-    disjoint aM k.r2 /\ disjoint aM k.n /\
-    bn_v h aM < bn_v h k.n)
+    disjoint a (k.r2 <: lbignum t k.len) /\ disjoint a (k.n <: lbignum t k.len) /\
+    disjoint aM (k.r2 <: lbignum t k.len) /\ disjoint aM (k.n <: lbignum t k.len) /\
+    bn_v h aM < bn_v #t #k.len h k.n)
   (ensures  fun h0 _ h1 -> modifies (loc a) h0 h1 /\
-    bn_v h1 a < bn_v h0 k.n /\
+    bn_v h1 a < bn_v #t #k.len h0 k.n /\
     as_seq h1 a == S.bn_from_field (as_ctx h0 k) (as_seq h0 aM))
 
 
 inline_for_extraction noextract
-val bn_from_field: km:BM.mont U64 -> k:bn_mont_ctx{k.len == km.BM.bn.BN.len} -> bn_from_field_st k
+val bn_from_field: #t:limb_t -> km:BM.mont t -> k:bn_mont_ctx t{k.len == km.BM.bn.BN.len} -> bn_from_field_st k
 
 
 inline_for_extraction noextract
-let bn_field_add_st (k:bn_mont_ctx) =
-    aM:lbignum U64 k.len
-  -> bM:lbignum U64 k.len
-  -> cM:lbignum U64 k.len ->
+let bn_field_add_st (#t:limb_t) (k:bn_mont_ctx t) =
+    aM:lbignum t k.len
+  -> bM:lbignum t k.len
+  -> cM:lbignum t k.len ->
   Stack unit
   (requires fun h ->
     bn_mont_ctx_inv h k /\ live h aM /\ live h bM /\ live h cM /\
     eq_or_disjoint aM bM /\ eq_or_disjoint aM cM /\ eq_or_disjoint bM cM /\
-    disjoint k.n aM /\ disjoint k.n bM /\ disjoint k.n cM /\
-    bn_v h aM < bn_v h k.n /\ bn_v h bM < bn_v h k.n)
+    disjoint (k.n <: lbignum t k.len) aM /\
+    disjoint (k.n <: lbignum t k.len) bM /\
+    disjoint (k.n <: lbignum t k.len) cM /\
+    bn_v h aM < bn_v #t #k.len h k.n /\
+    bn_v h bM < bn_v #t #k.len h k.n)
   (ensures  fun h0 _ h1 -> modifies (loc cM) h0 h1 /\
-    bn_v h1 cM < bn_v h0 k.n /\
+    bn_v h1 cM < bn_v #t #k.len h0 k.n /\
     as_seq h1 cM == S.bn_field_add (as_ctx h0 k) (as_seq h0 aM) (as_seq h0 bM))
 
 
 inline_for_extraction noextract
-val bn_field_add: km:BM.mont U64 -> k:bn_mont_ctx{k.len == km.BM.bn.BN.len} -> bn_field_add_st k
+val bn_field_add: #t:limb_t -> km:BM.mont t -> k:bn_mont_ctx t{k.len == km.BM.bn.BN.len} -> bn_field_add_st k
 
 
 inline_for_extraction noextract
-let bn_field_sub_st (k:bn_mont_ctx) =
-    aM:lbignum U64 k.len
-  -> bM:lbignum U64 k.len
-  -> cM:lbignum U64 k.len ->
+let bn_field_sub_st (#t:limb_t) (k:bn_mont_ctx t) =
+    aM:lbignum t k.len
+  -> bM:lbignum t k.len
+  -> cM:lbignum t k.len ->
   Stack unit
   (requires fun h ->
     bn_mont_ctx_inv h k /\ live h aM /\ live h bM /\ live h cM /\
     eq_or_disjoint aM bM /\ eq_or_disjoint aM cM /\ eq_or_disjoint bM cM /\
-    disjoint k.n aM /\ disjoint k.n bM /\ disjoint k.n cM /\
-    bn_v h aM < bn_v h k.n /\ bn_v h bM < bn_v h k.n)
+    disjoint (k.n <: lbignum t k.len) aM /\
+    disjoint (k.n <: lbignum t k.len) bM /\
+    disjoint (k.n <: lbignum t k.len) cM /\
+    bn_v h aM < bn_v #t #k.len h k.n /\
+    bn_v h bM < bn_v #t #k.len h k.n)
   (ensures  fun h0 _ h1 -> modifies (loc cM) h0 h1 /\
-    bn_v h1 cM < bn_v h0 k.n /\
+    bn_v h1 cM < bn_v #t #k.len h0 k.n /\
     as_seq h1 cM == S.bn_field_sub (as_ctx h0 k) (as_seq h0 aM) (as_seq h0 bM))
 
 
 inline_for_extraction noextract
-val bn_field_sub: km:BM.mont U64 -> k:bn_mont_ctx{k.len == km.BM.bn.BN.len} -> bn_field_sub_st k
+val bn_field_sub: #t:limb_t -> km:BM.mont t -> k:bn_mont_ctx t{k.len == km.BM.bn.BN.len} -> bn_field_sub_st k
 
 
 inline_for_extraction noextract
-let bn_field_mul_st (k:bn_mont_ctx) =
-    aM:lbignum U64 k.len
-  -> bM:lbignum U64 k.len
-  -> cM:lbignum U64 k.len ->
+let bn_field_mul_st (#t:limb_t) (k:bn_mont_ctx t) =
+    aM:lbignum t k.len
+  -> bM:lbignum t k.len
+  -> cM:lbignum t k.len ->
   Stack unit
   (requires fun h ->
     bn_mont_ctx_inv h k /\ live h aM /\ live h bM /\ live h cM /\
     eq_or_disjoint aM bM /\ eq_or_disjoint aM cM /\ eq_or_disjoint bM cM /\
-    disjoint cM k.n /\
-    bn_v h aM < bn_v h k.n /\ bn_v h bM < bn_v h k.n)
+    disjoint cM (k.n <: lbignum t k.len) /\
+    bn_v h aM < bn_v #t #k.len h k.n /\
+    bn_v h bM < bn_v #t #k.len h k.n)
   (ensures  fun h0 _ h1 -> modifies (loc cM) h0 h1 /\
-    bn_v h1 cM < bn_v h0 k.n /\
+    bn_v h1 cM < bn_v #t #k.len h0 k.n /\
     as_seq h1 cM == S.bn_field_mul (as_ctx h0 k) (as_seq h0 aM) (as_seq h0 bM))
 
 
 inline_for_extraction noextract
-val bn_field_mul: km:BM.mont U64 -> k:bn_mont_ctx{k.len == km.BM.bn.BN.len} -> bn_field_mul_st k
+val bn_field_mul: #t:limb_t -> km:BM.mont t -> k:bn_mont_ctx t{k.len == km.BM.bn.BN.len} -> bn_field_mul_st k
 
 
 inline_for_extraction noextract
-let bn_field_sqr_st (k:bn_mont_ctx) =
-    aM:lbignum U64 k.len
-  -> cM:lbignum U64 k.len ->
+let bn_field_sqr_st (#t:limb_t) (k:bn_mont_ctx t) =
+    aM:lbignum t k.len
+  -> cM:lbignum t k.len ->
   Stack unit
   (requires fun h ->
     bn_mont_ctx_inv h k /\ live h aM /\ live h cM /\
-    eq_or_disjoint aM cM /\ disjoint cM k.n /\
-    bn_v h aM < bn_v h k.n)
+    eq_or_disjoint aM cM /\ disjoint cM (k.n <: lbignum t k.len) /\
+    bn_v h aM < bn_v #t #k.len h k.n)
   (ensures  fun h0 _ h1 -> modifies (loc cM) h0 h1 /\
-    bn_v h1 cM < bn_v h0 k.n /\
+    bn_v h1 cM < bn_v #t #k.len h0 k.n /\
     as_seq h1 cM == S.bn_field_sqr (as_ctx h0 k) (as_seq h0 aM))
 
 
 inline_for_extraction noextract
-val bn_field_sqr: km:BM.mont U64 -> k:bn_mont_ctx{k.len == km.BM.bn.BN.len} -> bn_field_sqr_st k
+val bn_field_sqr: #t:limb_t -> km:BM.mont t -> k:bn_mont_ctx t{k.len == km.BM.bn.BN.len} -> bn_field_sqr_st k
 
 
 inline_for_extraction noextract
-let bn_field_one_st (k:bn_mont_ctx) = oneM:lbignum U64 k.len ->
+let bn_field_one_st (#t:limb_t) (k:bn_mont_ctx t) = oneM:lbignum t k.len ->
   Stack unit
   (requires fun h ->
     bn_mont_ctx_inv h k /\ live h oneM /\
-    disjoint k.n oneM /\ disjoint k.r2 oneM)
+    disjoint (k.n <: lbignum t k.len) oneM /\
+    disjoint (k.r2 <: lbignum t k.len) oneM)
   (ensures  fun h0 _ h1 -> modifies (loc oneM) h0 h1 /\
-    bn_v h1 oneM < bn_v h0 k.n /\
+    bn_v h1 oneM < bn_v #t #k.len h0 k.n /\
     as_seq h1 oneM == S.bn_field_one (as_ctx h0 k))
 
 
 inline_for_extraction noextract
-val bn_field_one: km:BM.mont U64 -> k:bn_mont_ctx{k.len == km.BM.bn.BN.len} -> bn_field_one_st k
+val bn_field_one: #t:limb_t -> km:BM.mont t -> k:bn_mont_ctx t{k.len == km.BM.bn.BN.len} -> bn_field_one_st k
 
 
 inline_for_extraction noextract
-let bn_field_inv_st (k:bn_mont_ctx) =
-    aM:lbignum U64 k.len
-  -> aInvM:lbignum U64 k.len ->
+let bn_field_inv_st (#t:limb_t) (k:bn_mont_ctx t) =
+    aM:lbignum t k.len
+  -> aInvM:lbignum t k.len ->
   Stack unit
   (requires fun h ->
     bn_mont_ctx_inv h k /\ live h aM /\ live h aInvM /\
-    disjoint aM aInvM /\ disjoint k.n aM /\
-    disjoint k.n aInvM /\ disjoint k.r2 aInvM /\
-    0 < bn_v h aM /\ bn_v h aM < bn_v h k.n)
+    disjoint aM aInvM /\
+    disjoint (k.n <: lbignum t k.len) aM /\
+    disjoint (k.n <: lbignum t k.len) aInvM /\
+    disjoint (k.r2 <: lbignum t k.len) aInvM /\
+    0 < bn_v h aM /\ bn_v h aM < bn_v #t #k.len h k.n)
   (ensures  fun h0 _ h1 -> modifies (loc aInvM) h0 h1 /\
-    bn_v h1 aInvM < bn_v h0 k.n /\
+    bn_v h1 aInvM < bn_v #t #k.len h0 k.n /\
     as_seq h1 aInvM == S.bn_field_inv (as_ctx h0 k) (as_seq h0 aM))
 
 
 inline_for_extraction noextract
-val bn_field_inv: km:BM.mont U64 -> k:bn_mont_ctx{k.len == km.BM.bn.BN.len} -> bn_field_inv_st k
+val bn_field_inv: #t:limb_t -> km:BM.mont t -> k:bn_mont_ctx t{k.len == km.BM.bn.BN.len} -> bn_field_inv_st k
