code/bignum/Hacl.GenericField64.fsti
@@ -7,6 +7,12 @@ module GF = Hacl.Bignum.GenericField
 
 #set-options "--z3rlimit 50 --fuel 0 --ifuel 0"
 
+inline_for_extraction noextract
+let t_limbs: Hacl.Bignum.Definitions.limb_t = Lib.IntTypes.U64
+
+inline_for_extraction noextract
+let bn_mont_ctx_u64 = GF.bn_mont_ctx t_limbs
+
 [@@ CPrologue
 "/*******************************************************************************
 
@@ -14,7 +20,7 @@ A verified field arithmetic library.
 
 This is a 64-bit optimized version, where bignums are represented as an array
 of `len` unsigned 64-bit integers, i.e. uint64_t[len].
-All the arithmetic operations are performed in the Montgomery domen.
+All the arithmetic operations are performed in the Montgomery domain.
 
 *******************************************************************************/\n";
 Comment "Allocate and initialize a montgomery context.
@@ -33,12 +39,12 @@ Comment "Allocate and initialize a montgomery context.
 
   • n is a prime // needed for the modular multiplicative inverse
 "]
-val field_init: len:BN.meta_len Lib.IntTypes.U64 -> GF.bn_field_init_st len
+val field_init: len:BN.meta_len t_limbs -> GF.bn_field_init_st t_limbs len
 
 [@@ Comment "Return a size of the modulus `n` in limbs.
 
   The argument k is a montgomery context obtained through Hacl_GenericField64_field_init."]
-val field_get_len: k:GF.bn_mont_ctx -> GF.bn_field_get_len_st k
+val field_get_len: k:bn_mont_ctx_u64 -> GF.bn_field_get_len_st k
 
 [@@ Comment "Convert a bignum to its Montgomery representation.
 
@@ -51,7 +57,7 @@ val field_get_len: k:GF.bn_mont_ctx -> GF.bn_field_get_len_st k
   from Hacl.Spec.Bignum.GenericField.fsti, which amounts to:
   • a < n
 "]
-val to_field: k:GF.bn_mont_ctx -> GF.bn_to_field_st k
+val to_field: k:bn_mont_ctx_u64 -> GF.bn_to_field_st k
 
 [@@ Comment "Convert the result back from the Montgomery representation to the regular representation.
 
@@ -65,7 +71,7 @@ val to_field: k:GF.bn_mont_ctx -> GF.bn_to_field_st k
   from Hacl.Spec.Bignum.GenericField.fsti, which amounts to:
   • aM < n
 "]
-val from_field: k:GF.bn_mont_ctx -> GF.bn_from_field_st k
+val from_field: k:bn_mont_ctx_u64 -> GF.bn_from_field_st k
 
 [@@ Comment "Write `aM + bM mod n` in `cM`.
 
@@ -76,7 +82,7 @@ val from_field: k:GF.bn_mont_ctx -> GF.bn_from_field_st k
   from Hacl.Spec.Bignum.GenericField.fsti, which amounts to:
   • aM < n
   • bM < n "]
-val add: k:GF.bn_mont_ctx -> GF.bn_field_add_st k
+val add: k:bn_mont_ctx_u64 -> GF.bn_field_add_st k
 
 [@@ Comment "Write `aM - bM mod n` to `cM`.
 
@@ -87,7 +93,7 @@ val add: k:GF.bn_mont_ctx -> GF.bn_field_add_st k
   from Hacl.Spec.Bignum.GenericField.fsti, which amounts to:
   • aM < n
   • bM < n "]
-val sub: k:GF.bn_mont_ctx -> GF.bn_field_sub_st k
+val sub: k:bn_mont_ctx_u64 -> GF.bn_field_sub_st k
 
 [@@ Comment "Write `aM * bM mod n` in `cM`.
 
@@ -98,7 +104,7 @@ val sub: k:GF.bn_mont_ctx -> GF.bn_field_sub_st k
   from Hacl.Spec.Bignum.GenericField.fsti, which amounts to:
   • aM < n
   • bM < n "]
-val mul: k:GF.bn_mont_ctx -> GF.bn_field_mul_st k
+val mul: k:bn_mont_ctx_u64 -> GF.bn_field_mul_st k
 
 [@@ Comment "Write `aM * aM mod n` in `cM`.
 
@@ -108,13 +114,13 @@ val mul: k:GF.bn_mont_ctx -> GF.bn_field_mul_st k
   This function is *UNSAFE* and requires C clients to observe bn_field_sqr
   from Hacl.Spec.Bignum.GenericField.fsti, which amounts to:
   • aM < n "]
-val sqr: k:GF.bn_mont_ctx -> GF.bn_field_sqr_st k
+val sqr: k:bn_mont_ctx_u64 -> GF.bn_field_sqr_st k
 
 [@@ Comment "Convert a bignum `one` to its Montgomery representation.
 
   The argument oneM is meant to be `len` limbs in size, i.e. uint64_t[len].
   The argument k is a montgomery context obtained through Hacl_GenericField64_field_init."]
-val one: k:GF.bn_mont_ctx -> GF.bn_field_one_st k
+val one: k:bn_mont_ctx_u64 -> GF.bn_field_one_st k
 
 [@@ Comment "Write `aM ^ (-1) mod n` in `aInvM`.
 
@@ -125,4 +131,4 @@ val one: k:GF.bn_mont_ctx -> GF.bn_field_one_st k
   from Hacl.Spec.Bignum.GenericField.fsti, which amounts to:
   • aM < n
   • 0 < aM "]
-val inverse: k:GF.bn_mont_ctx -> GF.bn_field_inv_st k
+val inverse: k:bn_mont_ctx_u64 -> GF.bn_field_inv_st k
